examples/steel/CQueue.fsti
@@ -1,0 +1,54 @@
+module CQueue
+open Steel.Memory
+open Steel.Effect.Atomic
+open Steel.Effect
+open Steel.FractionalPermission
+open Steel.Reference
+module L = FStar.List.Tot
+
+val t (a: Type0) : Tot Type0
+
+noextract
+val v (a: Type0) : Tot Type0
+
+noextract
+val datas (#a: Type0) (l: v a) : Tot (list a)
+
+val queue (#a: Type) (x: t a) (l: Ghost.erased (v a)) : Tot (slprop u#1)
+
+val create_queue (a: Type) : Steel (t a & Ghost.erased (v a)) emp (fun x -> queue (fst x) (snd x))
+  (requires (fun _ -> True))
+  (ensures (fun _ res _ -> datas (snd res) == []))
+
+val enqueue
+  (#a: Type)
+  (x: t a)
+  (l: Ghost.erased (v a))
+  (w: a)
+: Steel (Ghost.erased (v a))
+    (queue x l)
+    (fun res -> queue x res)
+    (requires (fun _ -> True))
+    (ensures (fun _ res _ -> datas res == datas l `L.append` [w]))
+
+val queue_is_empty
+  (#a: Type)
+  (x: t a)
+  (l: Ghost.erased (v a))
+: Steel bool
+    (queue x l)
+    (fun _ -> queue x l)
+    (requires (fun _ -> True))
+    (ensures (fun _ res _ ->
+      res == Nil? (datas l)
+    ))
+
+val dequeue
+  (#a: Type)
+  (x: t a)
+  (l: Ghost.erased (v a))
+: Steel (a & Ghost.erased (v a))
+    (queue x l)
+    (fun res -> queue x (snd res))
+    (requires (fun _ -> Cons? (datas l) == true))
+    (ensures (fun _ res _ -> datas l == fst res :: datas (snd res)))
